cesm.v
@@ -19,6 +19,8 @@ Definition stack := list (closure + nat).
 Inductive configuration : Type :=
   | conf : heap → stack → closure → configuration.
 
+Definition I (e : expr) : configuration := conf nil nil (close e 0).
+
 Notation " x ↦ M " := (x, M) (at level 40).
 Notation " ⟨ Φ ⟩ m " := (conf Φ m) (at level 40).
 Notation " ⟨ Ψ , b ⟩ N " :=  (conf (cons b Ψ) N) (at level 40).
@@ -31,8 +33,6 @@ Fixpoint clu (v env:nat) (h:heap) : option nat := match v with
     | None => None
     end
   end.
-
-Definition domain (h:heap) : list nat := @map (nat * cell) nat (@fst nat cell) h.
 
 Definition fresh (n : nat) (h : heap) := 
   ~ In n (domain h).
@@ -73,6 +73,7 @@ Definition replaceClosure (l:nat) (c:closure) : nat * cell → nat * cell :=
     | (l', cl c' e) => if eq_nat_dec l l' then (l, cl c e) else x
     end.
 
+(*
 Definition step : {c1 | well_formed c1} → {c2 | well_formed c2}.
 refine (
   fun c1 => match c1 with
@@ -95,58 +96,7 @@ refine (
     end
   end
 ).
-split. 
-destruct x. 
-destruct p. 
+*)
 
-Reserved Notation " c1 '⇓' c2 " (at level 50).
-Inductive step : configuration → configuration → Prop :=
-  | Id : ∀ M B x y z Φ Ψ Υ v e, 
-                  cactus_lookup v z (Υ ++ (x ↦ {M,y} :: Φ)) x →
-              ⟨Φ, (x ↦ {M,y}), Υ⟩M ⇓ ⟨Ψ, (x ↦ {M,y}), Υ⟩close (:λB) e →
-    ⟨Φ, x ↦ {M, y}, Υ⟩close (var v) z ⇓ ⟨Ψ, x ↦ {close (:λB) e, y}, Υ⟩close (:λB) e
-  | Abs : ∀ N Φ e, ⟨Φ⟩close (:λN) e ⇓ ⟨Φ⟩close (:λN) e
-  | App : ∀ N M B B' Φ Ψ Υ f e ne ae, fresh f Ψ → 
-          ⟨Φ⟩close M e ⇓ ⟨Ψ⟩close (:λB) ne → 
-      ⟨Ψ, f ↦ {close N e, ne}⟩close B f ⇓ ⟨Υ⟩close (:λB') ae   →
-              ⟨Φ⟩close (M@N) e ⇓ ⟨Υ⟩close (:λB') ae
-where " c1 '⇓' c2 " := (step c1 c2).
-
-Lemma well_formed_inf : ∀ c x c' n  Φ Υ, well_formed (⟨Φ, x ↦ cl c' n, Υ⟩c) → 
-  well_formed (⟨Φ, x ↦ cl c' n, Υ⟩c').
-  intros. split. inversion H. unfold well_formed_heap in H1. apply forevery_app in H1.
-  destruct H1. simpl in H2. destruct H2. auto. 
-  auto. inversion H. auto. Qed. 
-
-Lemma cactus_lookup_inf : ∀ v x y m n e Φ Υ, cactus_lookup v x (Φ ++ (y ↦ {m, n}) :: Υ) e → ∀ M, cactus_lookup v x (Φ ++ (y ↦ {M, n}) :: Υ) e.
-intros. 
-
-
-Lemma inf_well_formed : ∀ c x c' n  Φ Υ, well_formed (⟨Φ, x ↦ cl c' n, Υ⟩c) → 
-  well_formed (⟨Φ, x ↦ cl c n, Υ⟩c).
-  intros. inversion H. split. induction Υ. simpl. destruct c. induction (fvs e).
-  simpl. auto. simpl. 
-  destruct (eq_nat_dec x n0). simpl. unfold domain. rewrite
-  map_app. simpl. unfold domain in H0. rewrite map_app in H0. simpl in H0. 
-  kapply forevery_app in H1. destruct H1. simpl in
-  H2. destruct H2. unfold closed_under in H0. clear H1 H2 H3.  (inversion H. apply forevery_app in H1.
-  auto. inversion H. auto. Qed. 
-
-Theorem well_formed_step : ∀ c v, well_formed c → c ⇓ v → well_formed v.
-intros. induction H0. apply well_formed_inf in H. apply IHstep in H.  
-
-Lemma values_only : ∀ c e M Ψ, c ⇓ ⟨Ψ⟩close M e → value M.
-intros. inversion H; simpl; auto. Qed.
-
-Example simple : (step (⟨nil⟩ close (:λ0 @ :λ0) 0) (⟨nil, 0 ↦ {close (:λ0) 0,
-0}⟩ close (:λ0) 0)).
-apply App with 0 nil 0 0.
-unfold fresh. simpl.  auto. 
-apply Abs.
-rewrite <- app_nil_l with (prod nat cell) (cons (0↦{close (:λ0) 0, 0}) nil).
-apply Id.
-apply zero.
-apply Abs. 
-Qed.
 
 
