compiler.v
@@ -1,28 +1,16 @@
-Require expr expr_db_nat.
+Require expr expr_db_nat cbn cem cesm.
 Require Import db util assembly.
 Require Import Arith.Peano_dec.
 Require Import List Datatypes.
+Require Import Unicode.Utf8.
 
 (* Function instead of logical relation, not equivalent! Function takes first
 value in environment, logical relation takes any. Logical relation wrong? *)
 
-Fixpoint db (tm : expr.tm) (env : list (nat * nat)) : option expr_db_nat.expr := match tm with 
-  | expr.var v => match lookup eq_nat_dec v env with
-    | Some v' => Some (expr_db_nat.var v')
-    | None => None
-    end
-  | expr.abs v b => match db b ((v, 0):: map (fmap' S) env) with 
-    | Some b' => Some (expr_db_nat.lam b')
-    | None => None
-    end
-  | expr.app m n => match db m env with
-    | Some m' => match db n env with 
-      | Some n' => Some (expr_db_nat.app m' n')
-      | None => None
-      end
-    | None => None
-    end
-  end.
+(*
+Axiom refl_trans_iso : ∀ e e' m, expr.closed e → cbn.step (cbn.i e) e' → 
+                assembly.step (assembly.i (compile e)) m ∧ m ≃ e'.
+*)
 
 (* TODO: Assembler from db terms.
 Fixpoint assemble (e : expr_db_nat.expr) : program. *)
