db.v
@@ -9,53 +9,45 @@ Set Implicit Arguments.
 
 (* db.v : used to relate debruijn terms with standard terms *) 
 
-Definition fmap {A B C} (f : B -> C) : A * B -> A * C  := fun x => match x with
-  | (a, b) => (a, f b) end. 
-
 Definition fmap' {A B C} (f : A -> C) : A * B -> C * B  := fun x => match x with
   | (a, b) => (f a, b) end. 
 
 (* a relation between standard lambda terms and deBruijn-indexed term, note that
   standard variables are nats as well *)
-Inductive db : expr.tm -> list (prod nat nat) -> expr_db_nat.expr -> Prop :=
-  | dbVar : forall bs cs v i, 
-      db (expr.var v) (bs ++ (v, i) :: cs) (expr_db_nat.var i)
-  | dbAbs : forall bs v b b',
-      db b ((v,0) :: map (fmap S) bs) b' ->
-      db (expr.abs v b) bs (expr_db_nat.lam b')
-  | dbApp : forall m n m' n' bs,
-      db m bs m' ->
-      db n bs n' ->
-      db (expr.app m n) bs (expr_db_nat.app m' n').
+Fixpoint db (tm : expr.tm) (env : Map nat nat) : option expr_db_nat.expr := match tm with 
+  | expr.var v => match lookup eq_nat_dec v env with
+    | Some v' => Some (expr_db_nat.var v')
+    | None => None
+    end
+  | expr.abs v b => match db b ((v, 0):: map (fmap S) env) with 
+    | Some b' => Some (expr_db_nat.lam b')
+    | None => None
+    end
+  | expr.app m n => match db m env with
+    | Some m' => match db n env with 
+      | Some n' => Some (expr_db_nat.app m' n')
+      | None => None
+      end
+    | None => None
+    end
+  end.
 
-Axiom dbf : {t | expr.closed t} -> {e | expr_db_nat.closed e}.
+(* TODO
+Lemma dbClosedUnder (tm : expr.tm) (env : Map nat nat) : 
+  subset (expr.fvs tm) (domain env) → exists e, db tm env = Some e.
+intros. induction tm. apply subset_domain_map with (l:=(expr.fvs (expr.var n)))
+(eq0:=eq_nat_dec) in H. simpl in H. simpl. destruct H. destruct H. rewrite H.
+apply ex_intro with (expr_db_nat.var x). reflexivity. simpl in H. rewrite
+app_subset_and in H. destruct H. apply IHtm1 in H. apply IHtm2 in H0. simpl.
+destruct H, H0. rewrite H. rewrite H0. apply ex_intro with (expr_db_nat.app x
+x0). reflexivity. simpl in H. simpl. rewrite <- subset_remove_cons in H. 
+rewrite <- domain_fmap with (C:=nat) (f:=S) in H. 
+induction (expr.fvs tm).
+assert (subset nil (domain env)). apply subset_nil. apply IHtm in H0. destruct
+H0. apply ex_intro with (expr_db_nat.lam x). 
+*)
 
-(* debruijn relation for closed terms *)
-Definition deBruijn (t:expr.tm) (e:expr_db_nat.expr) : Prop := db t nil e.
-
-Lemma let_inline :forall (b c:prod nat nat),
-    (fst (let a := b in c)) = (let a := b in fst c).
-    auto. Qed.
-
-Definition domain (A B : Type) : list (prod A B) -> list A := map (@fst A B). 
-
-Lemma domain_fmap : forall A B C (f:B->C) (xs:list (A * B)),  domain (map
-(fmap f) xs) = domain xs.
-intros. induction xs. crush. crush. Qed. 
-
-Theorem db_closed_under : forall f t e, db t f e -> subset (expr.fvs t) (domain f).
-intros.  induction H.  simpl.  unfold domain.  rewrite map_app.  simpl.
-split.  apply in_or_app.  simpl.  right. left.  reflexivity.  apply I.  simpl.
-simpl in IHdb.  rewrite domain_fmap in IHdb. rewrite <-
-subset_remove_cons. assumption. simpl. apply app_subset_and. split; assumption.
-Qed. 
-
-Theorem db_closed : forall t e, db t nil e -> expr.fvs t = nil.
-intros. apply db_closed_under in H. simpl in H. unfold subset in H. destruct
-(expr.fvs t).  reflexivity. inversion H. inversion H0. Qed. 
-
-Axiom closed_db_under : forall f t, subset (expr.fvs t) (domain f) -> 
-  exists e, db t f e.
+Definition alpha_equiv (t1 t2 : expr.tm) : Prop := db t1 = db t2.
 
 (*
 Theorem closed_db_under : forall f t, subset (expr.fvs t) (domain f) -> exists
@@ -72,36 +64,5 @@ right. crush. crush. rewrite <- subset_remove_cons. rewrite domain_fmap in IHdb.
 assumption. simpl. apply app_subset_and. crush. Qed. 
 *)
 
-Definition lookup' {A B} : forall (f : list (A * B)) (a: {a | In a (domain f)}), B. 
-intros. induction f. crush. destruct a. inversion f. destruct a0. assumption.
-Qed.
-
-Definition In' {A} := flip (@In A).
-
-Definition sumbool_or {A B} : {A} + {B} -> A \/ B := fun b => match b with
-  | left a => or_introl a
-  | right b => or_intror b
-  end.
-
-Definition inx (x:nat) := In x (domain ((0,1) :: nil)).
-
-Lemma in_heap : forall (A B : Type) (k : A) (f : list (prod A B)), In k (domain f)
-                         -> (exists v, In (k,v) f).
-intros. unfold domain in H. apply in_map_iff with (prod A B) A (@fst A B) f k in
-H. destruct H.  destruct H. destruct H. destruct x. simpl. apply ex_intro with
-b. assumption. Qed. 
-
-(* id = id *) Lemma ex1 : db (expr.abs 0 (expr.var 0)) nil (expr_db_nat.lam (expr_db_nat.var 0)).
-apply dbAbs. simpl. rewrite <- app_nil_l with (prod nat nat) ((0, 0) :: nil).
-apply dbVar. Qed.
-
-(* true = true *)
-Lemma ex2 : db (expr.abs 0 (expr.abs 1 (expr.var 0))) nil 
-               (expr_db_nat.lam (expr_db_nat.lam (expr_db_nat.var 1))).
-apply dbAbs.
-apply dbAbs. simpl. rewrite <- app_nil_l with (prod nat nat) ((0, 1) :: nil). 
-rewrite app_comm_cons.
-apply dbVar.
-Qed.
 
 
